$$\begin{eqnarray}
条件: \quad
&①& \quad S_{n}(x)=\sum\limits_{k=1}^{n}u_{k}(x)为\sum\limits_{n=1}^{\infty}u_{n}(x)的\textcolor{orange}{\underline{\textbf{前n项和}}} 
\end{eqnarray}$$
$$给定\quad S_{1}(x) \ , \ \cdots \ , \ S_{n}(x) \ , \ \cdots$$
$$\quad \Updownarrow \quad$$
>$$S_{1}(x)=\sum\limits_{k=1}^{1}u_{k}(x)=u_{1}(x)$$
>$$S_{2}(x)=\sum\limits_{k=1}^{2}u_{k}(x)=u_{1}(x)+u_{2}(x)$$
>$$S_{3}(x)=\sum\limits_{k=1}^{3}u_{k}(x)=u_{1}(x)+ \cdots +u_{3}(x)$$
>$$\vdots$$
>$$S_{n}(x)= \sum\limits_{k=1}^{n}u_{k}(x)= u_{1}(x) + \cdots + u_{n}(x)$$
>$$\vdots$$


$$记为\ : \quad \{S_{n}(x)\}$$


$$\{S_{n}(x)\} \ \  \overset{\triangle}{=} \ \ \sum\limits_{n=1}^{\infty}u_{n}(x)的一个\textcolor{orange}{\underline{\textbf{函数序列}}}$$
