$$\sum\limits_{n=1}^{\infty} \frac{x^{n}}{n^{p}}$$
### 问题

$$Qs: \qquad \sum\limits_{n=1}^{\infty} \frac{x^{n}}{n^{p}}的\textcolor{pink}{\underline{\textbf{收敛域}}}$$
### 求解

#### 收敛区间

$$\lim\limits_{n \rightarrow \infty} \frac{n^{p}}{(n+1)^{p}} = \lim\limits_{n \rightarrow \infty} \left(\frac{n}{n+1}\right)^{p} =  \left(\lim\limits_{n \rightarrow \infty}\frac{n}{n+1}\right) ^{p} = 1^{p} =1$$
$$\quad \Downarrow \quad $$
$$r = \frac{1}{\rho}= \frac{1}{1} =1 $$
$$\quad \Downarrow \quad $$
$$\textcolor{pink}{\underline{\textbf{收敛区间}}}为:\qquad (-1,1)$$

#### 收敛端点
##### $x=1$
$$\sum\limits_{n=1}^{\infty} \frac{1}{n^{p}}$$

###### $p >1$

$$\sum\limits_{n=1}^{\infty} \frac{1}{n^{p}} \ \sim \ \sum\limits_{n=1}^{\infty} \frac{1}{n^{2}}$$
$$\quad \Downarrow \quad $$


$$\sum\limits_{n=1}^{\infty} \frac{1}{n^{2}} \quad \textcolor{red}{\underline{\textbf{收敛}}}$$
$$\quad \Updownarrow \quad$$
$$\sum\limits_{n=1}^{\infty} \frac{1}{n^{p}} \quad \textcolor{red}{\underline{\textbf{收敛}}}$$
###### $p=1$

$$\sum\limits_{n=1}^{\infty} \frac{1}{n} \quad \textcolor{orange}{\underline{\textbf{发散}}}$$
$$\quad \Updownarrow \quad$$

$$\sum\limits_{n=1}^{\infty}  \frac{1}{n^{p}} \quad \textcolor{orange}{\underline{\textbf{发散}}}$$
###### $p<1$

$$\sum\limits_{n=1}^{\infty} \frac{1}{n^{p}} \ \sim \  \sum\limits_{n=1}^{\infty} \frac{1}{n^{\frac{1}{2}}}$$
$$\quad \Downarrow \quad $$
$$\sum\limits_{n=1}^{\infty} \frac{1}{n^{\frac{1}{2}}} \quad \textcolor{orange}{\underline{\textbf{发散}}}$$
$$\quad \Updownarrow \quad$$

$$\sum\limits_{n=1}^{\infty} \frac{1}{n^{p}} \quad \textcolor{orange}{\underline{\textbf{发散}}}$$

##### $x=-1$

$$\sum\limits_{n=1}^{\infty} \frac{(-1)^{n}}{n^{p}}$$
###### $p>0$

$$\sum\limits_{n=1}^{\infty} \frac{(-1)^{n}}{n^{p}}$$
$$\quad \Downarrow \quad $$
$$\textcolor{pink}{\underline{\textbf{交错级数}}}的Lebniz判别法$$
$$\quad \Downarrow \quad $$
$$\sum\limits_{n=1}^{\infty} \frac{(-1)^{n}}{n^{p}} \quad \textcolor{red}{\underline{\textbf{收敛}}}$$

###### $p=0$

$$\sum\limits_{n=1}^{\infty} (-1)^{n}$$
$$\quad \Downarrow \quad $$
$$\textcolor{pink}{\underline{\textbf{交错级数}}}$$
$$\quad \Downarrow \quad $$
$$\sum\limits_{n=1}^{\infty} \frac{(-1)^{n}}{n^{p}} \quad \textcolor{orange}{\underline{\textbf{发散}}}$$
###### $p<0$

也就是

$$-p>0$$
因此

$$\sum\limits_{n=1}^{\infty} (-1)^{n} \cdot n^{-p}$$
$$\quad \Downarrow \quad $$
$$\tag{核心手法}\lim\limits_{n \rightarrow \infty} (-1)^{n} \cdot n^{-p}  \ \neq \ 0$$
$$\quad \Downarrow \quad $$
$$\sum\limits_{n=1}^{\infty} (-1)^{n} \cdot n^{-p} \quad \textcolor{orange}{\underline{\textbf{发散}}}$$



#### 综上所述

###### $p>1$

$$\textcolor{pink}{\underline{\textbf{收敛域}}}为:\qquad [-1,1]$$
###### $0<p  \leqslant 1$

$$\textcolor{pink}{\underline{\textbf{收敛域}}}为:\qquad [-1,1)$$
###### $p  \leqslant0$

$$\textcolor{pink}{\underline{\textbf{收敛域}}}为:\qquad (-1,1)$$
$$\qquad QED\ !$$